\begin{enumerate}
	\item
	$$
	\begin{aligned}
	{R_{yx}}\left( \tau  \right) & = {R_{xx}}\left( \tau  \right)*h\left( \tau  \right)\\
	& = \int\limits_{ - \infty }^{ + \infty } {{e^{j\alpha \left( {\tau  - z} \right)}}h\left( z \right)dz} \\
	& = {e^{j\alpha \tau }}\int\limits_{ - \infty }^{ + \infty } {{e^{ - j\alpha z}}h\left( z \right)dz} \\
	& = {e^{j\alpha \tau }}H\left( \alpha  \right)
	\end{aligned}
	$$
	
	برای مورد دوم داریم:
	
	$$
	\begin{aligned}
	{R_{yy}}\left( \tau  \right) & = {R_{yx}}\left( \tau  \right) * {h^*}\left( { - \tau } \right)\\
	& = H\left( \alpha  \right)\int\limits_{ - \infty }^{ + \infty } {{e^{j\alpha \left( {\tau  - z} \right)}}{h^*}\left( { - z} \right)dz} \\
	& = H\left( \alpha  \right){e^{j\alpha \tau }}\int\limits_{ - \infty }^{ + \infty } {{e^{ - j\alpha z}}{h^*}\left( { - z} \right)dz} \\
	& = H\left( \alpha  \right){e^{j\alpha \tau }}{H^*}\left( \alpha  \right)\\
	& = {e^{j\alpha \tau }}{\left| {H\left( \alpha  \right)} \right|^2}
	\end{aligned}
	$$	
	
	\item
	
	$$
	\begin{aligned}
		{R_{yx}}\left( {{t_1},{t_2}} \right) & = {R_{xx}}\left( {{t_1},{t_2}} \right) * h\left( {{t_1}} \right)\\
		& = \int\limits_{ - \infty }^{ + \infty } {{e^{j\left( {\alpha \left( {{t_1} - z} \right) - \beta {t_2}} \right)}}h\left( z \right)dz} \\
		& = {e^{j\left( {\alpha {t_1} - \beta {t_2}} \right)}}\int\limits_{ - \infty }^{ + \infty } {{e^{ - j\alpha z}}h\left( z \right)dz} \\
		& = {e^{j\left( {\alpha {t_1} - \beta {t_2}} \right)}}H\left( \alpha  \right)
	\end{aligned}
	$$
	
	برای مورد دوم داریم:
	
	$$
	\begin{aligned}
		{R_{yy}}\left( {{t_1},{t_2}} \right) & = {R_{yx}}\left( {{t_1},{t_2}} \right) * {h^*}\left( {{t_2}} \right)\\
		& = H\left( \alpha  \right)\int\limits_{ - \infty }^{ + \infty } {{e^{j\left( {\alpha {t_1} - \beta \left( {{t_2} - z} \right)} \right)}}{h^*}\left( z \right)dz} \\
		& = H\left( \alpha  \right){e^{j\left( {\alpha {t_1} - \beta {t_2}} \right)}}\int\limits_{ - \infty }^{ + \infty } {{e^{j\beta z}}{h^*}\left( z \right)dz} \\
		& = {e^{j\left( {\alpha {t_1} - \beta {t_2}} \right)}}H\left( \alpha  \right){H^*}\left( \beta  \right)
	\end{aligned}
	$$
\end{enumerate}